SepLogic.v
@@ -1,0 +1,210 @@
+
+Require Export Imp.
+
+(* First we define syntax of the language *)
+
+(* We could reuse aexp and bexp defined for Imp. *)
+
+(* Redefine commands here. To distinguish them 
+   from Imp commands, we call them scom *)
+(* You need to change it into an inductive definition *)
+Definition scom : Type := admit.
+
+
+(* Program states, which is called sstate *)
+Definition store := id -> nat.
+
+(* if heap maps a natural number (address) to
+   None, we say the address is not a valid address,
+   or it is not in the domain of the heap *)
+Definition heap := nat -> option nat.
+
+Axiom functional_extensionality : forall {X Y: Type} {f g : X -> Y},
+    (forall (x: X), f x = g x) ->  f = g.
+
+(* Define an empty heap, which contains no memory cells *)
+Definition emp_heap : heap := 
+  fun (l: nat) => None.
+
+Definition in_dom (l: nat) (h: heap) : Prop :=
+  exists n, h l = Some n.
+
+Definition not_in_dom (l: nat) (h: heap) : Prop :=
+  h l = None.
+
+Theorem in_not_in_dec : 
+  forall l h, {in_dom l h} + {not_in_dom l h}.
+Proof.
+  intros l h. unfold in_dom. unfold not_in_dom.
+  destruct (h l).
+  left. exists n. auto.
+  right. auto.
+Defined.
+
+(* h1 and h2 have disjoint domain *)
+Definition disjoint (h1 h2: heap) : Prop := 
+  forall l, not_in_dom l h1 \/ not_in_dom l h2.
+
+(* union of two heaps *)
+Definition h_union (h1 h2: heap) : heap :=
+  fun l => 
+    if (in_not_in_dec l h1) then h1 l else h2 l.
+
+(* h1 is a subset of h2 *)
+Definition h_subset (h1 h2: heap) : Prop := 
+  forall l n, h1 l = Some n -> h2 l = Some n.
+
+(* store update *)
+Definition st_update (s: store) (x: id) (n: nat) : store :=
+  fun x' => if eq_id_dec x x' then n else s x'.
+
+(* heap update *)
+Definition h_update (h: heap) (l: nat) (n: nat) : heap :=
+  fun l' => if eq_nat_dec l l' then Some n else h l'.
+
+Definition sstate := (store * heap) %type.
+
+(* since program may abort, we extend our state
+   definition to add a special state Abt *)
+Inductive ext_state : Type :=
+  St:  sstate -> ext_state    (* normal state *)
+| Abt: ext_state.             (* abort *)
+
+
+(* Next we define the operational semantics *)
+
+(* big-step semantics. You should change it into 
+   an inductive definition *)
+Definition big_step: 
+   scom * sstate -> ext_state -> Prop := admit.
+
+(* small-step semantics. Should be inductive too *)
+Definition small_step: 
+   scom * ext_state -> scom * ext_state -> Prop 
+  := admit.
+
+
+(** Assertions **)
+Definition sass := sstate -> Prop.
+
+(* define semantics of assertion emp *)
+Definition emp : sass := 
+    fun st: sstate => 
+      snd st = emp_heap.
+
+(* assertion e1 |-> e2 *)
+Definition pto (e1 e2: aexp) : sass := 
+    fun st: sstate =>
+      match st with
+      | (s, h) => h = h_update emp_heap (aeval s e1) (aeval s e2)
+      end.
+Notation "e1 '|->' e2" := (pto e1 e2) (at level 60).
+
+(* p * q *)
+Definition star (p q : sass) : sass := 
+    fun st: sstate =>
+      match st with
+      | (s, h) => 
+        exists h1, exists h2, 
+          disjoint h1 h2 /\ h_union h1 h2 = h /\ p (s, h1) /\ q (s, h2)
+      end.
+Notation "p '**' q" := (star p q) (at level 70).
+
+(* p --* q *)
+Definition simp (p q: sass) : sass := 
+  fun (st : sstate) =>
+    match st with
+    | (s, h) => 
+      forall h', disjoint h' h -> p (s, h') -> q (s, h_union h h')
+    end.
+Notation "p '--*' q" := (simp p q) (at level 80).
+
+
+Definition pure (p: sass) : Prop := 
+  forall s h1 h2, p (s, h1) -> p (s, h2).
+
+Definition precise (p: sass) : Prop := 
+  forall h h1 h2 s, 
+     h_subset h1 h 
+     -> h_subset h2 h 
+     -> p (s, h1) 
+     -> p (s, h2)
+     -> h1 = h2.
+
+Definition intuitionistic (p: sass) : Prop := 
+  forall s h h', p (s, h) -> disjoint h h' -> p (s, h_union h h').
+
+
+(* continue here *)
+
+Definition s_conj (p q: sass) : sass :=
+  fun (s: sstate) => p s /\ q s.
+Notation "p '//\\' q" := (s_conj p q) (at level 75).
+
+Definition s_disj (p q: sass) : sass :=
+  fun (s: sstate) => p s \/ q s.
+Notation "p '\\//' q" := (s_disj p q) (at level 78).
+
+Definition s_imp (p q: sass) : sass :=
+  fun (s: sstate) => p s -> q s.
+Notation "p '~~>' q" := (s_imp p q) (at level 85).
+
+Definition strongerThan (p q: sass) : Prop :=
+  forall s: sstate, s_imp p q s.
+Notation "p '==>' q" := (strongerThan p q) (at level 90).
+
+Definition spEquiv (p q: sass) : Prop :=
+  (p ==> q) /\ (q ==> p).
+Notation "p '<==>' q" := (spEquiv p q) (at level 90).
+
+(* Prove the following lemmas *)
+Lemma disj_star_distr: forall (p q r: sass),
+  (p \\// q) ** r <==> (p ** r) \\// (q ** r).
+Admitted.  
+
+Lemma conj_star_distr: forall (p q r: sass),
+  (p //\\ q) ** r ==> (p ** r) //\\ (q ** r).
+Admitted.
+
+Lemma precise_conj_distr: forall (p q r: sass),
+  precise r -> (p ** r) //\\ (q ** r) ==> (p //\\ q) ** r.
+Admitted.
+ 
+Inductive multiStep : 
+    scom * ext_state -> scom * ext_state -> Prop :=
+| step0: forall c s, multiStep (c, s) (c, s)
+| stepn: forall c s c' s' c'' s'', 
+           small_step (c, s) (c', s')
+           -> multiStep (c', s') (c'', s'')
+           -> multiStep (c, s) (c'', s'').
+
+(* c is safe at state s *)
+Definition safeAt (c: scom) (s: sstate) : Prop :=
+(* ~ multiStep (c, St s) Abt *) 
+(*
+forall c' s',
+  multiStep (c, St s) (c', St s')
+  -> c' = SKIP \/ exists c'', exists s'', small_step (c', St s') (c'', St s'').
+*)
+admit.
+
+Definition safeMono (c: scom) : Prop := 
+(*
+  forall s h h', 
+    safeAt c (s, h) -> disjoint h h' -> safeAt c (s, h_union h h').
+*)
+admit.
+
+Definition frame (c: scom) : Prop :=
+  forall s h1 h2 c' s' h',
+    safeAt c (s, h1) 
+    -> disjoint h1 h2 
+    -> small_step (c, St (s, h_union h1 h2)) (c', St (s', h'))
+    -> exists h1', 
+         small_step (c, St (s, h1)) (c', St (s', h1'))
+         /\ disjoint h1' h2 
+         /\ h_union h1' h2 = h'.
+
+Theorem locality: forall c : scom, safeMono c /\ frame c.
+Admitted.
+
