lf/Imp.v
@@ -1415,6 +1415,7 @@ Proof.
   inversion Heval. subst. clear Heval. simpl.
   apply t_update_eq.  Qed.
 
+
 (** **** Exercise: 3 stars, recommended (XtimesYinZ_spec)  *)
 (** State and prove a specification of [XtimesYinZ]. *)
 
